total for Pi/Prop can be shown without needing irrel

PIW.v
@@ -192,24 +192,6 @@ Proof using.
 Abort.
 
 
-Definition Prop_R3 {A B : Prop} (R : A -> B -> Prop) : Prop 
- := (A <-> B) /\ (forall a b, R a b).
-
-Require Import ProofIrrelevance.
-
-
-Lemma Prop_R2Spec {A₁ A₂: Prop} (R : A₁ -> A₂ -> Prop):
-  TotalHeteroRel R <=> Prop_R3 R.
-Proof using.
-  intros. split; intros Hyp;
-  unfold Prop_R3; unfold TotalHeteroRel, TotalHeteroRelHalf, rInv in *.
-- destruct Hyp. split.
-  + split; intros a; try destruct (s a);  try destruct (s0 a); eauto.
-  + intros. destruct (s a).
-    pose proof (proof_irrelevance _ x b). subst. assumption.
-- intros. destruct Hyp. split; intros a; firstorder; eauto.
-Qed.
-
 
 (* iff implies TotalHeteroRel -- we should return the relation \r1 r2 => True *)
 Definition IWP_RP2
